ulib/experimental/Steel.ST.HigherArray.fsti
@@ -43,6 +43,7 @@ val base_len (#elt: Type) (b: base_t elt) : GTot nat
 val ptr ([@@@strictly_positive] elt: Type u#a) : Type0
 [@@noextract_to "krml"]
 val null_ptr (elt: Type u#a) : ptr elt
+
 // TODO: turn into a stateful operation to avoid comparing dangling pointers
 val is_null_ptr (#elt: Type u#a) (p: ptr elt) : Pure bool
   (requires True)
@@ -58,6 +59,10 @@ val ptr_base_offset_inj (#elt: Type) (p1 p2: ptr elt) : Lemma
     p1 == p2
   ))
 
+val base_len_null_ptr (elt: Type u#a) : Lemma
+  (base_len (base (null_ptr elt)) == 0)
+  [SMTPat (base_len (base (null_ptr elt)))]
+
 /// A concrete type to represent a C array, as a C pointer and a ghost
 /// array length.  By virtue of the length being ghost, Karamel will
 /// extract this type as just ptr, but to inline the definition of
@@ -70,7 +75,8 @@ let array ([@@@strictly_positive] elt: Type u#a) : Tot Type0 =
 
 inline_for_extraction
 [@@noextract_to "krml"]
-val null (#a: Type0) : array a
+let null (#a: Type u#a) : array a
+= (| null_ptr a, Ghost.hide 0 |)
 
 /// This will extract to "let p = a"
 inline_for_extraction
@@ -81,6 +87,13 @@ let ptr_of
 : Tot (ptr elt)
 = match a with // dfst is not marked inline_for_extraction, so we need to reimplement it
   | (| p, _ |) -> p
+
+inline_for_extraction
+[@@noextract_to "krml"]
+let is_null (#a: Type u#a) (p: array a) : Pure bool
+  (requires True)
+  (ensures (fun res -> res == true <==> p == null))
+= is_null_ptr (ptr_of p)
 
 let length (#elt: Type) (a: array elt) : GTot nat =
   dsnd a
